Wip

lean-circuit/LeanCircuit/SemanticEquivalence.lean
@@ -12,6 +12,25 @@ variable [Fact (Nat.Prime Order)]
 
 abbrev D := 20
 
+def recover_tail {depth : Nat} {F: Type} (H: Hash F 2) (ix : Vector (Option Dir) depth) (proof : Vector F depth) (item : F) : Option F := match depth with
+  | Nat.zero => item
+  | Nat.succ _ =>
+    let pitem := proof.head
+    match ix.head with
+      | some Dir.left => recover_tail H ix.tail proof.tail (H vec![item, pitem])
+      | some Dir.right => recover_tail H ix.tail proof.tail (H vec![pitem, item])
+      | none => none
+
+def recover {depth : Nat} {F: Type} (H : Hash F 2) (ix : Vector (Option Dir) depth) (proof : Vector F depth) (item : F) : Option F := match depth with
+  | Nat.zero => item
+  | Nat.succ _ =>
+    let pitem := proof.head
+    let recover' := recover H ix.tail proof.tail item
+    match ix.head, recover' with
+      | some Dir.left, some r => H vec![r, pitem]
+      | some Dir.right, some r => H vec![pitem, r]
+      | _ , _ => none
+
 def embed_dir : Dir -> F
   | x => Dir.toZMod x
 
@@ -21,12 +40,13 @@ def embed_dir_vector {depth} (ix: Vector Dir depth) : Vector F depth :=
 lemma dir_embed_recover {d : Dir} : Dir.nat_to_dir (embed_dir d).val = d := by
   cases d <;> rfl
 
+def vec_dir_to_option {depth} (ix: Vector Dir depth) : Vector (Option Dir) depth := Vector.map (fun x => some x) ix
+
 @[simp]
 lemma dir_embed_recover_vector {depth} (ix: Vector Dir depth) :
-  Dir.create_dir_vec (embed_dir_vector ix) = ix := by
+  Dir.create_dir_vec (embed_dir_vector ix) = vec_dir_to_option ix := by
+  unfold vec_dir_to_option
   simp [Dir.create_dir_vec, embed_dir_vector, dir_embed_recover]
-  apply Vector.eq
-  simp
 
 @[simp]
 lemma embed_dir_vector_reverse {depth} (ix : Vector Dir depth) :
@@ -57,17 +77,44 @@ lemma Poseidon2_uncps (a b : F) (k : F -> Prop) : Semaphore.Poseidon2 a b k ↔ 
     simp [Semaphore.Poseidon2, poseidon₂, poseidon_3_correct, getElem]
     rfl
 
+def MerkleTreeRecoverHash (dir hash sibling: F) : Option F :=
+  match p: Dir.nat_to_dir dir.val with
+    | Dir.left => some (poseidon₂ vec![hash, sibling])
+    | Dir.right => some (poseidon₂ vec![sibling, hash])
+    | none => none
+
+@[simp]
+def MerkleTreeRecoverHash_is_some {dir hash sibling: F} :
+  (is_bit dir) → (∃y, (MerkleTreeRecoverHash dir hash sibling) = some y) := by
+    intros
+    rename_i h
+    unfold MerkleTreeRecoverHash
+    --unfold Dir.nat_to_dir at h
+    unfold Dir.nat_to_dir
+    induction ZMod.val dir generalizing h with
+    | zero =>
+      simp
+    | succ x _ =>
+      induction x generalizing h with
+      | zero => simp
+      | succ _ _ =>
+        simp
+        sorry
+
 lemma MerkleTreeRecoverRound_uncps {dir hash sibling : F} {k : F -> Prop}:
     Semaphore.MerkleTreeRecoverRound dir hash sibling k ↔
-    is_bit dir ∧ k (match Dir.nat_to_dir dir.val with
-    | Dir.left => poseidon₂ vec![hash, sibling]
-    | Dir.right => poseidon₂ vec![sibling, hash]) := by
+    is_bit dir ∧ (∃y, (MerkleTreeRecoverHash dir hash sibling) = some y ∧ k y) := by
     simp [Semaphore.MerkleTreeRecoverRound, Gates.is_bool]
     intro hb
     rw [Poseidon2_uncps, Poseidon2_uncps]
     cases hb <;> {
+        unfold MerkleTreeRecoverHash
         simp [*, Gates.select, Gates.is_bool, Dir.nat_to_dir]
-        try rfl
+        rename_i h
+        subst_vars
+        unfold ZMod.val
+        unfold Order
+        simp
     }
 
 def merkle_tree_recover_rounds (Leaf : F) (PathIndices Siblings : Vector F n) (k : F -> Prop) : Prop :=
@@ -76,21 +123,32 @@ def merkle_tree_recover_rounds (Leaf : F) (PathIndices Siblings : Vector F n) (k
   | Nat.succ _ => Semaphore.MerkleTreeRecoverRound PathIndices.head Leaf Siblings.head fun next =>
     merkle_tree_recover_rounds next PathIndices.tail Siblings.tail k
 
+@[simp]
+def merkle_tree_recover_rounds_uncps_is_some
+  {Leaf : F}
+  {PathIndices Siblings : Vector F n}:
+  is_vector_binary PathIndices → (∃x, recover_tail poseidon₂ (Dir.create_dir_vec PathIndices) Siblings Leaf = some x) := by sorry
+
 lemma merkle_tree_recover_rounds_uncps
   {Leaf : F}
   {PathIndices Siblings : Vector F n}
   {k : F -> Prop}:
-  merkle_tree_recover_rounds Leaf PathIndices Siblings k ↔
-  is_vector_binary PathIndices ∧ k (MerkleTree.recover_tail poseidon₂ (Dir.create_dir_vec PathIndices) Siblings Leaf) := by
-  induction PathIndices, Siblings using Vector.inductionOn₂ generalizing Leaf with
+  merkle_tree_recover_rounds Leaf PathIndices Siblings k ↔ is_vector_binary PathIndices ∧
+  (∃x, recover_tail poseidon₂ (Dir.create_dir_vec PathIndices) Siblings Leaf = some x) ∧ k x := by
+  induction PathIndices, Siblings using Vector.inductionOn₂ generalizing x Leaf with
   | nil =>
     simp [is_vector_binary]
-    rfl
-  | @cons n ix sib ixes sibs ih =>
+    unfold merkle_tree_recover_rounds
+    sorry
+    --unfold recover_tail    
+    --simp
+    -- rfl
+  | @cons n ix sib ixes sibs ih =>    
+    simp [*] at ih
     simp [MerkleTree.recover_tail_reverse_equals_recover, MerkleTree.recover_tail, merkle_tree_recover_rounds]
     simp [MerkleTreeRecoverRound_uncps, is_vector_binary_cons, and_assoc, ih]
     intros
-    rfl
+    sorry
 
 lemma MerkleTreeInclusionProof_looped (Leaf: F) (PathIndices: Vector F D) (Siblings: Vector F D) (k: F -> Prop):
     Semaphore.MerkleTreeInclusionProof_20_20 Leaf PathIndices Siblings k =
@@ -103,9 +161,11 @@ lemma MerkleTreeInclusionProof_looped (Leaf: F) (PathIndices: Vector F D) (Sibli
     rfl
 
 lemma MerkleTreeInclusionProof_20_20_uncps {Leaf : F} {PathIndices Siblings : Vector F D} {k : F -> Prop}:
-    Semaphore.MerkleTreeInclusionProof_20_20 Leaf PathIndices Siblings k ↔
-    is_vector_binary PathIndices ∧ k (MerkleTree.recover_tail poseidon₂ (Dir.create_dir_vec PathIndices) Siblings Leaf) := by
-    simp [MerkleTreeInclusionProof_looped, merkle_tree_recover_rounds_uncps]
+    Semaphore.MerkleTreeInclusionProof_20_20 Leaf PathIndices Siblings k ↔ is_vector_binary PathIndices ∧
+    (∃x, recover_tail poseidon₂ (Dir.create_dir_vec PathIndices) Siblings Leaf = some x) ∧ k x := by
+    simp [MerkleTreeInclusionProof_looped]
+    simp [merkle_tree_recover_rounds_uncps]
+    sorry
 
 abbrev secret (IdentityNullifier: F) (IdentityTrapdoor: F) : F :=
   poseidon₂ vec![IdentityNullifier, IdentityTrapdoor]
@@ -116,10 +176,10 @@ abbrev identity_commitment (IdentityNullifier: F) (IdentityTrapdoor: F) : F :=
 abbrev nullifier_hash (ExternalNullifier: F) (IdentityNullifier: F) : F :=
   poseidon₂ vec![ExternalNullifier, IdentityNullifier]
 
-def circuit_sem (IdentityNullifier IdentityTrapdoor ExternalNullifier NullifierHash Root: F) (Path Proof: Vector F D): Prop :=
+def circuit_sem (IdentityNullifier IdentityTrapdoor ExternalNullifier NullifierHash Root: F) (Path Proof: Vector F D) : Prop :=
     NullifierHash = nullifier_hash ExternalNullifier IdentityNullifier ∧
     is_vector_binary Path ∧
-    MerkleTree.recover poseidon₂ (Dir.create_dir_vec Path).reverse Proof.reverse (identity_commitment IdentityNullifier IdentityTrapdoor) = Root
+    (∃x, recover poseidon₂ (Dir.create_dir_vec Path).reverse Proof.reverse (identity_commitment IdentityNullifier IdentityTrapdoor) = some x ∧ x = Root)
 
 theorem circuit_semantics {IdentityNullifier IdentityTrapdoor SignalHash ExternalNullifier NullifierHash Root: F} {Path Proof: Vector F D}:
     Semaphore.circuit IdentityNullifier IdentityTrapdoor Path Proof SignalHash ExternalNullifier NullifierHash Root ↔
@@ -145,8 +205,14 @@ theorem circuit_semantics {IdentityNullifier IdentityTrapdoor SignalHash Externa
       apply And.intro
       {rfl}
       apply And.intro
-      {assumption}
-      {rfl}
+      sorry
+      {
+        sorry
+        --assumption
+      }
+      -- {
+      --   rfl
+      -- }
     case mpr =>
       intro h
       cases h; rename_i h₁ h₂
@@ -158,5 +224,9 @@ theorem circuit_semantics {IdentityNullifier IdentityTrapdoor SignalHash Externa
       apply And.intro
       {rfl}
       apply And.intro
-      assumption
-      {rfl}
+      sorry
+      {
+        sorry
+      }
+      -- assumption
+      -- {rfl}
