lean-circuit/lakefile.lean
@@ -9,7 +9,7 @@ require mathlib from git
   "https://github.com/leanprover-community/mathlib4.git"@"ea67efc21e4e1496f0a1d954cd0c0a952523133a"
 
 require ProvenZK from git
-  "https://github.com/reilabs/proven-zk.git"@"v1.0.0"
+  "https://github.com/reilabs/proven-zk.git"@"a5da22e8421930d23a5c44e4c9c5693d606c6e81"
 
 lean_lib LeanCircuit {
   -- add library configuration options here
